Almost done. 3 more prop and one more function.

src/SmtyP.v
@@ -5,8 +5,10 @@ Require Import Context.
 Import Context.Context.
 Require Import Coq.Lists.List.
 Require Import Smty.
+Require Import LibTactics.
 
 Import Smty.Smty.
+
 
 
 Module SmtyP.
@@ -28,7 +30,7 @@ Fixpoint rcd_field_ty (rcd: list (id * ty)) (field : id) : option ty :=
 
 
 
-Inductive has_type : Context ty -> tm -> ty -> Prop :=
+Inductive has_type : Context -> tm -> ty -> Prop :=
 | ht_none : 
     forall ctx,
         has_type ctx tnone TNone
@@ -39,10 +41,10 @@ Inductive has_type : Context ty -> tm -> ty -> Prop :=
     has_type vctx fb T ->
     has_type vctx (tif crit tb fb) T
 | ht_var: forall ctx T i,
-    byContext ctx i = T ->
+    byContext ctx i = Some T ->
     has_type ctx (tvar i) T
-| ht_zero : forall ctx,
-    has_type ctx tzero TNat
+| ht_int : forall ctx n,
+    has_type ctx (tint n) TNat
 | ht_suc : forall ctx t,
     has_type ctx t TNat ->
     has_type ctx (tsuc t) TNat
@@ -52,25 +54,21 @@ Inductive has_type : Context ty -> tm -> ty -> Prop :=
 | ht_ngt : forall ctx t0 t1,
     has_type ctx t0 TNat ->
     has_type ctx t1 TNat ->
-    has_type ctx (ngt t0 t1) TBool
+    has_type ctx (tngt t0 t1) TBool
 | ht_nlt : forall ctx t0 t1,
     has_type ctx t0 TNat ->
     has_type ctx t1 TNat ->
-    has_type ctx (nlt t0 t1) TBool
+    has_type ctx (tnlt t0 t1) TBool
 | ht_neq : forall ctx t0 t1,
     has_type ctx t0 TNat ->
     has_type ctx t1 TNat ->
-    has_type ctx (neq t0 t1) TBool
-| ht_neq : forall ctx t0 t1,
-    has_type ctx t0 TNat ->
-    has_type ctx t1 TNat ->
-    has_type ctx (neq t0 t1) TBool
+    has_type ctx (tneq t0 t1) TBool
 | ht_chr : forall ctx n,
     has_type ctx (tchr n) TChr
 | ht_ceq : forall ctx t0 t1,
     has_type ctx t0 TChr ->
     has_type ctx t1 TChr ->
-    has_type ctx (ceq t0 t1) TBool
+    has_type ctx (tceq t0 t1) TBool
 | ht_fun : forall ctx i T body TO,
     has_type (update i T ctx) body TO ->
     has_type ctx (tfun i T body) (TFun T TO)
@@ -101,16 +99,228 @@ Inductive has_type : Context ty -> tm -> ty -> Prop :=
     has_type ctx tl (TFun TL TO) ->
     has_type ctx tr (TFun TR TO) ->
     has_type ctx (tcase crit tl tr) TO
-| ht_letrcd1 : forall ctx rcd tid suty TO,
+| ht_letrcd : forall ctx cons rcd tid suty body TO,
     subty (TRcd tid suty rcd) suty ->
-    has_type (update cons (rcd_cons_ty rcd tty) ctx) body TO ->
-    has_type ctx (tletrcd cons tid1 suty rcd body) TO
-| ht_field : forall ctx suty i,
+    has_type (update cons (rcd_cons_ty rcd (TRcd tid suty rcd)) ctx) body TO ->
+    has_type ctx (tletrcd cons tid suty rcd body) TO
+| ht_field : forall ctx rcd i tid suty T,
     rcd_field_ty rcd i = Some T ->
-    has_type (ht_field (TRcd tid suty rcd) i) (TFun (TRcd tid suty rcd) T)
+    has_type ctx (tfield (TRcd tid suty rcd) i) (TFun (TRcd tid suty rcd) T)
 | ht_seq : forall ctx t0 t1 T0 T1,
-    has_type t0 T0 ->
-    has_type t1 T1 ->
-    has_type (tseq t0 t1) T1.
+    has_type ctx t0 T0 ->
+    has_type ctx t1 T1 ->
+    has_type ctx (tseq t0 t1) T1.
+
+Hint Constructors has_type.
 
 
+Fixpoint nominal_typed (ctx: Context) (t : tm) : option ty :=
+    match t with
+    | tnone => Some TNone
+    | tif crit tb fb => 
+        match (nominal_typed ctx crit) with
+            | Some TBool => match (nominal_typed ctx tb), (nominal_typed ctx fb) with
+                            | Some a, Some b => if(eq_ty_dec a b) then Some a else None
+                            | _, _ => None
+                            end
+            | _ => None
+        end
+    | tvar i => byContext ctx i
+    | tint _ => Some TNat
+    | tsuc n => 
+        match (nominal_typed ctx n) with
+            | Some TNat => Some TNat
+            | _ => None
+        end
+    | tdec n =>
+        match (nominal_typed ctx n) with
+            | Some TNat => Some TNat
+            | _ => None
+        end
+    | tngt a b => 
+        match (nominal_typed ctx a), (nominal_typed ctx b) with
+            | Some TNat, Some TNat => Some TBool
+            | _, _ => None
+        end
+    | tnlt a b =>
+        match (nominal_typed ctx a), (nominal_typed ctx b) with
+            | Some TNat, Some TNat => Some TBool
+            | _, _ => None
+        end
+    | tneq a b =>
+        match (nominal_typed ctx a), (nominal_typed ctx b) with
+            | Some TNat, Some TNat => Some TBool
+            | _, _ => None
+        end
+    | tchr _ => Some TChr
+    | tceq a b =>
+        match (nominal_typed ctx a), (nominal_typed ctx b) with
+            | Some TChr, Some TChr => Some TBool
+            | _, _ => None
+        end   
+    | tfun i T body =>
+        match nominal_typed (update i T ctx) body with
+            | Some TO => Some (TFun T TO)
+            | _ => None
+        end
+    | tapp a b =>
+        match (nominal_typed ctx a), (nominal_typed ctx b) with
+            | Some (TFun i o), Some Ti => if(eq_ty_dec i Ti) then Some o else None
+            | _, _ => None
+        end
+    | tlet i T bind body =>
+        match (nominal_typed (update i T ctx) bind) with
+        | Some Tbind => if (eq_ty_dec T Tbind) then nominal_typed (update i T ctx) body else None
+        | _ => None
+        end
+    | ttrue => Some TBool
+    | tfalse => Some TBool
+    | tbeq a b=>
+        match (nominal_typed ctx a), (nominal_typed ctx b) with
+            | Some TBool, Some TBool => Some TBool
+            | _, _ => None
+        end   
+    | tleft t T =>
+        match (nominal_typed ctx t) with
+            | Some TL => Some (TSum TL T)
+            | _ => None
+        end
+    | tright T t =>
+        match (nominal_typed ctx t) with
+            | Some TR => Some (TSum T TR)
+            | _ => None
+        end
+    | tcase crit lb rb =>
+        match (nominal_typed ctx crit), (nominal_typed ctx lb), (nominal_typed ctx rb) with
+        | Some (TSum TL TR), Some (TFun TL0 TO0), Some (TFun TR0 TO1) =>
+            if (andb (eq_ty_dec_bool TL TL0) (andb (eq_ty_dec_bool TR TR0) (eq_ty_dec_bool TO0 TO1)) )
+            then Some TO0 else None
+        | _, _, _ => None
+        end
+    | tletrcd cons' T suTy rcd body =>
+        nominal_typed (update cons' (rcd_cons_ty rcd (TRcd T suTy rcd)) ctx) body
+    | tfield (TRcd a b rcd) i => 
+        match (rcd_field_ty rcd i) with
+        | Some TO => Some (TFun (TRcd a b rcd) TO)
+        | _ => None
+        end
+    | tfield _ _ => None
+    | tseq pre post =>
+        match nominal_typed ctx pre with
+        | Some _ => nominal_typed ctx post
+        | _ => None
+        end
+    end.
+
+Ltac keep_rewrite :=
+    match goal with
+    | h: _ = _ |- _ => rewrite h; clear h; keep_rewrite
+    | h: _ = _ |- _ => try rewrite <- h; clear h; keep_rewrite
+    | _ => idtac
+    end.
+
+Theorem typed__nominal_typed :
+    forall t T, 
+    has_type empty t T -> 
+    nominal_typed empty t = Some T.
+
+    intros t T h;
+    induction h; try (eauto; fail);
+
+    cbn; 
+    keep_rewrite; eauto using eq_ty_dec_id.
+
+    repeat (rewrite eq_ty_dec_bool_true). cbn. auto.
+Qed.
+
+Ltac destruct_match :=
+    match goal with
+    | h: match ?A with  _ => _  end = _ |- _ => destruct A; destruct_match; subst; eauto
+    | _ => idtac
+    end.
+
+Ltac apply_ctx ctx :=
+    match goal with
+    | h: forall x, _ |- _ => 
+        let x := fresh "h" in
+        (pose (h ctx) as x); generalize x; clear x; clear h; apply_ctx ctx
+    | _ => idtac
+    end; intros.
+
+Ltac destruct_match_keep :=
+    match goal with
+    | h: match ?A with  _ => _  end = _ |- _ => 
+        let k:= fresh in
+        destruct A eqn: k; destruct_match_keep
+    | _ => idtac
+    end.
+
+Ltac true_AND_has_to_be_true :=
+    match goal with
+    | h: (andb ?A  ?B) = true |- _ => 
+    let a := fresh "A" in
+    let b := fresh "B" in
+    destruct A eqn:a; 
+    destruct B eqn:b; 
+    try rewrite a in h; 
+    try rewrite b in h; 
+    eauto; cbn in h; 
+    try discriminate; 
+    generalize dependent h; true_AND_has_to_be_true
+    | _ => idtac
+    end; intros.
+
+Theorem nominal_typed__typed:
+    forall t ctx T, 
+    nominal_typed ctx t = Some T ->
+    has_type ctx t T.
+
+    intros t.
+    induction t; intros; eauto;
+    try (cbn in H;
+    apply_ctx ctx;
+        destruct_match;
+        try discriminate;
+        match goal with
+        | h : Some _ = Some _ |- _ => injection h; intros; subst; eauto
+        | _ => idtac
+        end; fail).
+    (* Case TFun. I am lazy with abstraction... *)
+    cbn in H.
+    poses' (IHt (update i t ctx)).
+    destruct_match.
+    injection H;intros ;subst;eauto.
+    try discriminate.
+
+    (* Case tlet *)
+    cbn in H.
+    poses' (IHt1 (update i t1 ctx)).
+    poses' (IHt2 (update i t1 ctx)).
+    destruct_match; try discriminate.
+
+    (* Case tcase *)
+    apply_ctx ctx.
+    cbn in H.
+    destruct_match_keep; subst; eauto;
+    try discriminate.
+    forwards: h;
+    forwards: h0;
+    forwards: h1; eauto.
+(*    let a := fresh "A" in
+    let b := fresh "B" in
+    destruct (eq_ty_dec_bool t0_1 t4_1) eqn:a; 
+    destruct (eq_ty_dec_bool t0_2 t5_1) eqn:b.
+    rewrite a in H6; 
+    rewrite b in H6; 
+    eauto; cbn in H6; 
+    try discriminate; 
+    generalize dependent H6.*)
+    true_AND_has_to_be_true.
+    
+    
+
+    
+    
+
+
+End SmtyP.
